LwRust.lean
@@ -1,5 +1,7 @@
 -- This module serves as the root of the `LwRust` library.
-import LwRust.CompleteProgram
+import LwRust.Core.Syntax
+import LwRust.Core.Proofs
+import LwRust.Core.ProgramSpace
 import LwRust.Extensions.Tuples
 import LwRust.Extensions.ControlFlow
 import LwRust.Extensions.Functions
